Generalizing the while laws.. adding theorems to designs.. adding while for Normal designs
git-svn-id: orca@498

C-verifier/src/Midend-IVL/Isabelle-UTP-Extended/theories/Design/utp_designs_more.thy
@@ -19,20 +19,36 @@ where "\<lceil>\<sigma>\<rceil>\<^sub>S\<^sub>D \<equiv> \<sigma> \<oplus>\<^sub
 abbreviation lift_usubst_des ("\<lceil>_\<rceil>\<^sub>s\<^sub>D")
 where "\<lceil>\<sigma>\<rceil>\<^sub>s\<^sub>D \<equiv> \<lceil>\<lceil>\<sigma>\<rceil>\<^sub>s\<rceil>\<^sub>S\<^sub>D"
 
-abbreviation drop_cpa_rel_des ("\<lfloor>_\<rfloor>\<^sub>S\<^sub>D")
+abbreviation drop_rel_usubst_des ("\<lfloor>_\<rfloor>\<^sub>S\<^sub>D")
 where "\<lfloor>\<sigma>\<rfloor>\<^sub>S\<^sub>D \<equiv> \<sigma> \<restriction>\<^sub>s (\<Sigma>\<^sub>D \<times>\<^sub>L \<Sigma>\<^sub>D)"
 
-abbreviation drop_cpa_des ("\<lfloor>_\<rfloor>\<^sub>s\<^sub>D")
-  where "\<lfloor>\<sigma>\<rfloor>\<^sub>s\<^sub>D \<equiv> \<lfloor>\<lfloor>\<sigma>\<rfloor>\<^sub>S\<^sub>D\<rfloor>\<^sub>s"
+abbreviation drop_usubst_des ("\<lfloor>_\<rfloor>\<^sub>s\<^sub>D")
+where "\<lfloor>\<sigma>\<rfloor>\<^sub>s\<^sub>D \<equiv> \<lfloor>\<lfloor>\<sigma>\<rfloor>\<^sub>S\<^sub>D\<rfloor>\<^sub>s"
 
 subsection {*UTP-Relations drop*}
 
-abbreviation drop_cpa_pre_uexpr ("\<lfloor>_\<rfloor>\<^sub><\<^sub>D")
+abbreviation drop_pre_uexpr_des ("\<lfloor>_\<rfloor>\<^sub><\<^sub>D")
 where "\<lfloor>P\<rfloor>\<^sub><\<^sub>D \<equiv> \<lfloor>\<lfloor>P\<rfloor>\<^sub>D\<rfloor>\<^sub><"
 
-abbreviation drop_cpa_post_uexpr ("\<lfloor>_\<rfloor>\<^sub>>\<^sub>D")
-  where "\<lfloor>P\<rfloor>\<^sub>>\<^sub>D \<equiv> \<lfloor>\<lfloor>P\<rfloor>\<^sub>D\<rfloor>\<^sub>>"    
-    
+abbreviation drop_post_uexpr_des ("\<lfloor>_\<rfloor>\<^sub>>\<^sub>D")
+where "\<lfloor>P\<rfloor>\<^sub>>\<^sub>D \<equiv> \<lfloor>\<lfloor>P\<rfloor>\<^sub>D\<rfloor>\<^sub>>"    
+
+section {*Normal Design setup*}
+
+abbreviation ndesign_lfp :: "('\<alpha> hrel_des \<Rightarrow> '\<alpha> hrel_des) \<Rightarrow> '\<alpha> hrel_des" ("\<mu>\<^sub>N") where
+"\<mu>\<^sub>N F \<equiv> \<^bold>\<mu>\<^bsub>NDES\<^esub> F"
+
+abbreviation ndesign_gfp :: "('\<alpha> hrel_des \<Rightarrow> '\<alpha> hrel_des) \<Rightarrow> '\<alpha> hrel_des" ("\<nu>\<^sub>N") where
+"\<nu>\<^sub>N F \<equiv> \<^bold>\<nu>\<^bsub>NDES\<^esub> F"
+
+syntax
+  "_ndmu" :: "pttrn \<Rightarrow> logic \<Rightarrow> logic" ("\<mu>\<^sub>N _ \<bullet> _" [0, 10] 10)
+  "_ndnu" :: "pttrn \<Rightarrow> logic \<Rightarrow> logic" ("\<nu>\<^sub>N _ \<bullet> _" [0, 10] 10)
+
+translations
+  "\<mu>\<^sub>N X \<bullet> P" == "\<^bold>\<mu>\<^bsub>CONST NDES\<^esub> (\<lambda> X. P)"
+  "\<nu>\<^sub>N X \<bullet> P" == "\<^bold>\<nu>\<^bsub>CONST NDES\<^esub> (\<lambda> X. P)"
+  
 section{*Control flow statements*}    
   
 subsection{*SKIP design*}  
@@ -51,45 +67,68 @@ where "bif\<^sub>D b then P else Q eif \<equiv> (P \<triangleleft> \<lceil>b\<rc
 
 subsection{*assert and assume*}
 
-definition assume_des :: "'\<alpha> upred \<Rightarrow> ('\<alpha>) hrel_des" ("_\<^sup>\<top>\<^sup>D" [999] 999) where
- [urel_defs]: "assume_des c \<equiv> (bif\<^sub>D c then SKIP\<^sub>D else \<top>\<^sub>D eif)"
+definition assume_des :: "'\<alpha> upred \<Rightarrow> ('\<alpha>) hrel_des" ("_\<^sup>\<top>\<^sup>D" [999] 999) 
+where [urel_defs]: "assume_des c \<equiv> (bif\<^sub>D c then SKIP\<^sub>D else \<top>\<^sub>D eif)"
 
-definition assert_des :: "'\<alpha> upred \<Rightarrow> ('\<alpha>) hrel_des" ("_\<^sub>\<bottom>\<^sub>D" [999] 999) where
- [urel_defs]: "assert_des c \<equiv> (bif\<^sub>D c then SKIP\<^sub>D else \<bottom>\<^sub>D eif)"
+definition assert_des :: "'\<alpha> upred \<Rightarrow> ('\<alpha>) hrel_des" ("_\<^sub>\<bottom>\<^sub>D" [999] 999) 
+where [urel_defs]: "assert_des c \<equiv> (bif\<^sub>D c then SKIP\<^sub>D else \<bottom>\<^sub>D eif)"
 
 subsection{*Scoping*}
 
-definition blockD ("bob\<^sub>D INIT (_) BODY /(_) RESTORE /(_) RETURN/(_) eob") where
-[urel_defs]:
+definition blockD ("bob\<^sub>D INIT (_) BODY /(_) RESTORE /(_) RETURN/(_) eob") 
+where [urel_defs]:
   "bob\<^sub>D INIT init BODY body RESTORE restore RETURN return eob= 
     Abs_uexpr (\<lambda>(s, s'). 
         \<lbrakk>init ;; body ;; 
          Abs_uexpr (\<lambda>(t, t').\<lbrakk>restore (s, s') (t, t');; return(s, s') (t, t')\<rbrakk>\<^sub>e (t, t'))\<rbrakk>\<^sub>e (s, s'))" 
-
-subsection{*Loops*}
+ 
+subsection{*Design Iterations*}
   
-definition While_gfp_des :: "'\<alpha> cond \<Rightarrow> ('\<alpha>) hrel_des \<Rightarrow> ('\<alpha>) hrel_des" ("while\<^sup>\<top>\<^sup>D _ do _ od") where
-"while\<^sup>\<top>\<^sup>D b do B od = (\<nu>\<^sub>D X \<bullet> bif\<^sub>D b then (B ;; X) else SKIP\<^sub>D eif)"
+definition While_gfp_des :: "'\<alpha> cond \<Rightarrow> '\<alpha> hrel_des \<Rightarrow> '\<alpha> hrel_des" ("while\<^sup>\<top>\<^sup>D _ do _ od")
+where "while\<^sup>\<top>\<^sup>D b do B od = (\<nu>\<^sub>D X \<bullet> bif\<^sub>D b then (B ;; X) else SKIP\<^sub>D eif)"
 
-
-definition While_lfp_des :: "'\<alpha> cond \<Rightarrow> ('\<alpha>) hrel_des \<Rightarrow> ('\<alpha>) hrel_des" ("while\<^sub>\<bottom>\<^sub>D _ do _ od") where
-"while\<^sub>\<bottom>\<^sub>D b do B od =  (\<mu>\<^sub>D X \<bullet> bif\<^sub>D b then (B ;; X) else SKIP\<^sub>D eif)"
+definition While_lfp_des :: "'\<alpha> cond \<Rightarrow> '\<alpha> hrel_des \<Rightarrow> '\<alpha> hrel_des" ("while\<^sub>\<bottom>\<^sub>D _ do _ od") 
+where "while\<^sub>\<bottom>\<^sub>D b do B od =  (\<mu>\<^sub>D X \<bullet> bif\<^sub>D b then (B ;; X) else SKIP\<^sub>D eif)"
 
 purge_notation while_top ("while _ do _ od")
 
-abbreviation While_bot_des :: "'\<alpha> cond \<Rightarrow> ('\<alpha>) hrel_des \<Rightarrow> ('\<alpha>) hrel_des" ("while _ do _ od") where
-"while b do B od \<equiv> while\<^sub>\<bottom>\<^sub>D b do B od"
+abbreviation While_bot_des :: "'\<alpha> cond \<Rightarrow> '\<alpha> hrel_des \<Rightarrow> '\<alpha> hrel_des" ("while\<^sub>D _ do _ od") 
+where "while\<^sub>D b do B od \<equiv> while\<^sub>\<bottom>\<^sub>D b do B od"
 
 subsection{*While-loop inv*}
 text {*While loops with invariant decoration*}
 
 purge_notation while_inv ("while _ invr _ do _ od" 71)
 
-definition While_inv_des :: "'\<alpha> cond \<Rightarrow> '\<alpha> cond \<Rightarrow> ('\<alpha>) hrel_des \<Rightarrow> ('\<alpha>) hrel_des" ("while _ invr _ do _ od") where
-"while b invr p do S od = while b do S od"
+definition While_inv_des :: "'\<alpha> cond \<Rightarrow> '\<alpha> cond \<Rightarrow> '\<alpha> hrel_des \<Rightarrow> '\<alpha> hrel_des" ("while\<^sub>D _ invr _ do _ od") 
+where "while\<^sub>D b invr p do S od = while\<^sub>D b do S od"
 
 declare While_gfp_des_def [urel_defs]
 declare While_inv_des_def [urel_defs]
 declare While_lfp_des_def [urel_defs]
-   
+
+subsection{*Normal Design Iterations*}   
+
+  
+definition While_gfp_ndes :: "'\<alpha> cond \<Rightarrow> '\<alpha> hrel_des \<Rightarrow> '\<alpha> hrel_des" ("while\<^sup>\<top>\<^sup>N _ do _ od")
+where "while\<^sup>\<top>\<^sup>N b do B od = (\<nu>\<^sub>N X \<bullet> bif\<^sub>D b then (B ;; X) else SKIP\<^sub>D eif)"
+
+definition While_lfp_ndes :: "'\<alpha> cond \<Rightarrow> '\<alpha> hrel_des \<Rightarrow> '\<alpha> hrel_des" ("while\<^sub>\<bottom>\<^sub>N _ do _ od") 
+where "while\<^sub>\<bottom>\<^sub>N b do B od =  (\<mu>\<^sub>N X \<bullet> bif\<^sub>D b then (B ;; X) else SKIP\<^sub>D eif)"
+
+abbreviation While_bot_ndes :: "'\<alpha> cond \<Rightarrow> '\<alpha> hrel_des \<Rightarrow> '\<alpha> hrel_des" ("while\<^sub>N _ do _ od") 
+where "while\<^sub>N b do B od \<equiv> while\<^sub>\<bottom>\<^sub>N b do B od"
+
+subsection{*While-loop inv*}
+text {*While loops with invariant decoration*}
+
+purge_notation while_inv ("while _ invr _ do _ od" 71)
+
+definition While_inv_ndes :: "'\<alpha> cond \<Rightarrow> '\<alpha> cond \<Rightarrow> '\<alpha> hrel_des \<Rightarrow> '\<alpha> hrel_des" ("while\<^sub>N _ invr _ do _ od") 
+where "while\<^sub>N b invr p do S od = while\<^sub>N b do S od"
+
+declare While_gfp_ndes_def [urel_defs]
+declare While_inv_ndes_def [urel_defs]
+declare While_lfp_ndes_def [urel_defs]
+
 end
