C-verifier/src/Midend-IVL/Isabelle-UTP/utp/utp.thy
@@ -21,6 +21,7 @@ imports
   utp_tactics
   "../../Isabelle-UTP-Extended/hoare/HoareLogic/PartialCorrectness/utp_hoare"
   "../../Isabelle-UTP-Extended/utp/utp_rec_total"
+  "../../Isabelle-UTP-Extended/utp/utp_sp"
   utp_wp
   utp_theory
   utp_concurrency
